SmallStep.v
@@ -1,52 +1,238 @@
 Require Import Common.
 Require Import Memory.
-Require Import Syntax.
+Require Import Value.
+Require Import Lang.
 Require Import State.
 Require Import BinNatDef.
+Require Import LoadStore.
+Require Import List.
+Require Import Bool.
+
 
 Module Ir.
 
-Definition sstep_det (c:Ir.Config.t) (i:Ir.inst): option Ir.Config.t :=
+Module SmallStep.
+
+Import Ir.Inst.
+
+
+Definition twos_compl (n:N) (sz:nat):N :=
+  N.modulo n (N.shiftl 2%N (N.of_nat sz)).
+
+Definition twos_compl2 (n:nat) (sz:nat):N :=
+  N.modulo (N.of_nat n) (N.shiftl 2%N (N.of_nat sz)).
+
+Definition twos_compl_add (x y:N) (sz:nat):N :=
+  twos_compl (N.add x y) sz.
+
+Definition twos_compl_sub (x y:N) (sz:nat):N :=
+  twos_compl (N.sub (N.add x (N.shiftl 2%N (N.of_nat sz))) y) sz.
+
+
+Definition p2N (p:Ir.ptrval) (m:Ir.Memory.t) (sz:nat):N :=
+  match p with
+  | Ir.plog (l, o) =>
+    match Ir.log_to_phy m l o with
+    | Some (Ir.pphy (o', _, _)) =>
+      twos_compl2 o' sz
+    | _ => 0%N
+    end
+  | Ir.pphy (o, _, _) =>
+    twos_compl2 o sz
+  end.
+
+Definition psub p1 p2 m bsz :=
+  let s := N.shiftl 2%N (N.of_nat bsz) in
+  match (p1, p2) with
+  | (Ir.plog (l1, o1), Ir.plog (l2, o2)) =>
+    if Nat.eqb l1 l2 then
+      Ir.num (twos_compl_sub (N.of_nat o1) (N.of_nat o2) bsz)
+    else Ir.poison
+  | (Ir.pphy (o1, _, _), Ir.plog _) =>
+    Ir.num (twos_compl_sub (N.of_nat o1) (p2N p2 m bsz) bsz)
+  | (Ir.plog _, Ir.pphy (o2, _, _)) =>
+    Ir.num (twos_compl_sub (p2N p1 m bsz) (N.of_nat o2) bsz)
+  | (Ir.pphy (o1, _, _), Ir.pphy (o2, _, _)) =>
+    Ir.num (twos_compl_sub (N.of_nat o1) (N.of_nat o2) bsz)
+  end.
+
+Definition gep (p:Ir.ptrval) (idx:N) (t:Ir.ty) (m:Ir.Memory.t): Ir.val :=
+  match p with
+  | Ir.plog (l, o) =>
+    match (Ir.Memory.get m l) with
+    | Some blk =>
+      let o' := (N.to_nat (twos_compl_add (N.of_nat o) idx Ir.PTRSZ)) in
+      if Ir.MemBlock.inbounds o blk &&
+         Ir.MemBlock.inbounds o' blk then Ir.ptr (Ir.plog (l, o'))
+      else Ir.poison (* out of bounds *)
+    | None => Ir.poison (* unreachable *)
+    end
+  | Ir.pphy (o, Is, cid) =>
+    Ir.ptr (Ir.pphy (o,
+                     (N.to_nat (twos_compl_add (N.of_nat o) idx Ir.PTRSZ))::Is, cid))
+  end.
+
+Definition free p m: option (Ir.Memory.t) :=
+  match p with
+  | Ir.plog (l, 0) => Ir.Memory.free m l
+  | Ir.pphy (o, Is, cid) =>
+    match (Ir.Memory.zeroofs_block m o) with
+    | None => None
+    | Some (bid, mb) =>
+      if Ir.deref m p 1 then (* to use Is, cid info *)
+        Ir.Memory.free m bid
+      else None
+    end
+  | _ => None
+  end.
+
+Definition to_num (b:bool): Ir.val :=
+  Ir.num (if b then 1%N else 0%N).
+
+(* Semantics of instructions which behave deterministically. *)
+Definition step_det (c:Ir.Config.t) (i:Ir.Inst.t)
+: option (Ir.event * Ir.Config.t) :=
   match i with
-  | Ir.iadd r (Ir.ity bsz) op1 op2 =>
-    Ir.Config.update_rval c r
+  | iadd r (Ir.ity bsz) op1 op2 =>
+    Some (Ir.e_none,
+      Ir.Config.update_rval c r
       match (Ir.Config.get_val c op1, Ir.Config.get_val c op2) with
       | (Some (Ir.num i1), Some (Ir.num i2)) =>
-        Ir.num (N.modulo (N.add i1 i2) (N.shiftl 2%N (N.of_nat bsz)))
+        Ir.num (twos_compl_add i1 i2 bsz)
       | (_, _) => Ir.poison
-      end
-  | Ir.isub r (Ir.ity bsz) op1 op2 =>
-    Ir.Config.update_rval c r
+      end)
+
+  | isub r (Ir.ity bsz) op1 op2 =>
+    Some (Ir.e_none,
+      Ir.Config.update_rval c r
       match (Ir.Config.get_val c op1, Ir.Config.get_val c op2) with
       | (Some (Ir.num i1), Some (Ir.num i2)) =>
-        Ir.num (N.modulo (N.sub (N.add i1 (N.shiftl 2%N (N.of_nat bsz))) i2)
-                                (N.shiftl 2%N (N.of_nat bsz)))
+        Ir.num (twos_compl_sub i1 i2 bsz)
       | (_, _) => Ir.poison
-      end
-  | Ir.ipsub r (Ir.ity bsz) (Ir.ptrty opty) op1 op2 =>
-    c
-  | Ir.igep r (Ir.ptrty retty) opptr opidx inb =>
-    c
-  | Ir.iload r retty opptr =>
-    c
-  | Ir.istore r valty opptr opval =>
-    c
-  | Ir.imalloc r blocksz =>
+      end)
+
+  | ipsub r (Ir.ity bsz) (Ir.ptrty opty) op1 op2 =>
+    Some (Ir.e_none,
+      Ir.Config.update_rval c r
+      match (Ir.Config.get_val c op1, Ir.Config.get_val c op2) with
+      | (Some (Ir.ptr p1), Some (Ir.ptr p2)) =>
+        psub p1 p2 (Ir.Config.m c) bsz
+      | (_, _) => Ir.poison
+      end)
+
+  | igep r (Ir.ptrty retty) opptr opidx inb =>
+    Some (Ir.e_none,
+      Ir.Config.update_rval c r
+      match (Ir.Config.get_val c opptr, Ir.Config.get_val c opidx) with
+      | (Some (Ir.ptr p), Some (Ir.num idx)) =>
+        gep p idx retty (Ir.Config.m c)
+      | (_, _) => Ir.poison
+      end)
+
+  | iload r retty opptr =>
+    match (Ir.Config.get_val c opptr) with
+    | (Some (Ir.ptr p)) =>
+      if Ir.deref (Ir.Config.m c) p (Ir.ty_bytesz retty) then
+        Some (Ir.e_none,
+              (Ir.Config.update_rval c r
+              (Ir.load_val (Ir.Config.m c) p retty)))
+      else None
+    | _ => None
+    end
+
+  | istore valty opptr opval =>
+    match (Ir.Config.get_val c opptr, Ir.Config.get_val c opval) with
+    | (Some (Ir.ptr p), Some v) =>
+      if Ir.deref (Ir.Config.m c) p (Ir.ty_bytesz valty) then
+        Some (Ir.e_none,
+              Ir.Config.update_m c (Ir.store_val (Ir.Config.m c) p v valty))
+      else None
+    | (_, _) => None
+    end
+
+  | imalloc r opty opval =>
     (* malloc is not determinstic! *)
     None
-  | Ir.ifree opptr =>
-    c
-  | Ir.iptrtoint r opptr (Ir.ity retty) =>
-    c
-  | Ir.iinttoptr r opint (Ir.ptrty retty) =>
-    c
-  | Ir.ievent opval =>
-    c
-  | Ir.iicmp_ptreq r opty opptr1 opptr2 =>
-    c
-  | Ir.iccmp_ptrule r opty opptr1 opttr2 =>
-    c
+
+  | ifree opptr =>
+    match (Ir.Config.get_val c opptr) with
+    | Some (Ir.ptr p) =>
+      match (free p (Ir.Config.m c)) with
+      | Some m => Some (Ir.e_none, Ir.Config.update_m c m)
+      | None => None
+      end
+    | _ => None
+    end
+
+  | iptrtoint r opptr (Ir.ity retty) =>
+    Some (Ir.e_none, Ir.Config.update_rval c r
+      match (Ir.Config.get_val c opptr) with
+      | Some (Ir.ptr p) => (Ir.num (p2N p (Ir.Config.m c) retty))
+      | _ => Ir.poison
+      end)
+
+  | iinttoptr r opint (Ir.ptrty retty) =>
+    Some (Ir.e_none, Ir.Config.update_rval c r
+      match (Ir.Config.get_val c opint) with
+      | Some (Ir.num n) =>
+        Ir.ptr (Ir.pphy (N.to_nat n, nil, None))
+      | _=> Ir.poison
+      end)
+
+  | ievent opval =>
+    match (Ir.Config.get_val c opval) with
+    | Some v => Some (Ir.e_some v, c)
+    | None => None
+    end
+
+  | iicmp_eq r opty op1 op2 =>
+    match (Ir.Config.get_val c op1, Ir.Config.get_val c op2) with
+    (* Integer comparison *)
+    | (Some (Ir.num n1), Some (Ir.num n2)) =>
+      Some (Ir.e_none, Ir.Config.update_rval c r (to_num (N.eqb n1 n2)))
+    (* Comparison with poison *)
+    | (Some (Ir.poison), _) =>
+      Some (Ir.e_none, Ir.Config.update_rval c r Ir.poison)
+    | (_, Some (Ir.poison)) =>
+      Some (Ir.e_none, Ir.Config.update_rval c r Ir.poison)
+    (* Pointer comparison *)
+    | (Some (Ir.ptr p1), Some (Ir.ptr p2)) =>
+      let m := Ir.Config.m c in
+      match (p1, p2) with
+      | (Ir.plog (l1, o1), Ir.plog (l2, o2)) =>
+        if Nat.eqb l1 l2 then
+          (* ICMP-PTR-LOGICAL *)
+          Some (Ir.e_none, Ir.Config.update_rval c r (to_num (Nat.eqb o1 o2)))
+        else
+          match (Ir.Memory.get m l1, Ir.Memory.get m l2) with
+          | (Some mb1, Some mb2) =>
+            (* ICMP-PTR-LOGICAL' *)
+            if Nat.leb o1 (Ir.MemBlock.n mb1) && Nat.leb o2 (Ir.MemBlock.n mb2) then
+              Some (Ir.e_none, Ir.Config.update_rval c r (to_num false))
+            else
+              (* ICMP-PTR-LOGICAL-NONDET-TRUE *)
+              None
+          | (_, _) => None
+          end
+      | (Ir.pphy (o1, Is1, cid1), _) =>
+        Some (Ir.e_none, Ir.Config.update_rval c r
+               (to_num (N.eqb (N.of_nat o1) (p2N p2 m Ir.PTRSZ))))
+      | (_, Ir.pphy (o2, Is2, cid2)) =>
+        Some (Ir.e_none, Ir.Config.update_rval c r
+               (to_num (N.eqb (p2N p1 m Ir.PTRSZ) (N.of_nat o2))))
+      end
+    | (_, _) => None (* In other cases, it is nondeterministic. *)
+    end
+
+  | iicmp_ule r opty opptr1 opttr2 =>
+    match (Ir.Config.get_val c opptr1, Ir.Config.get_val c opptr2) with
+    | (Some (Ir.num n1), Some (Ir.num n2)) =>
+      Nat.leb n1 n2
+    |
+
   | _ => None (* Untyped IR *)
   end.
+
+End SmallStep.
 
 End Ir.
