State.v
@@ -3,16 +3,16 @@ Require Import Lang.
 Require Import Memory.
 Require Import BinPos.
 Require Import List.
+Require Import Value.
 
 Module Ir.
 
-Inductive val :=
-| num: N -> val | ptr: Ir.ptrval -> val
-| poison: val.
-
-Definition regfile := list (nat * val).
+Definition regfile := list (nat * Ir.val).
 Definition stack := list Ir.callid.
 Definition pc := prod nat nat. (* block id, inst pos *)
+Inductive event :=
+| e_none: event
+| e_some (v:Ir.val): event.
 
 Module Config.
 
@@ -23,26 +23,29 @@ Structure t := mk
     cid_fresh: Ir.callid
   }.
 
-Definition get_rval (c:t) (regid:nat): option val :=
+Definition get_rval (c:t) (regid:nat): option Ir.val :=
   match (List.filter (fun x => Nat.eqb x.(fst) regid) c.(r)) with
   | nil => None
   | h::t => Some h.(snd)
   end.
 
-Definition get_val (c:t) (o:Ir.op): option val:=
+Definition get_val (c:t) (o:Ir.op): option Ir.val:=
   match o with
   | Ir.opconst c => Some
     match c with
-    | Ir.cnum cty cn => num cn
-    | Ir.cnullptr cty => ptr Ir.NULL
-    | Ir.cpoison cty => poison
-    | Ir.cglb glbvarid => ptr (Ir.plog (glbvarid, 0))
+    | Ir.cnum cty cn => Ir.num cn
+    | Ir.cnullptr cty => Ir.ptr Ir.NULL
+    | Ir.cpoison cty => Ir.poison
+    | Ir.cglb glbvarid => Ir.ptr (Ir.plog (glbvarid, 0))
     end
   | Ir.opreg regid => get_rval c regid
   end.
 
-Definition update_rval (c:t) (regid:nat) (v:val): t :=
+Definition update_rval (c:t) (regid:nat) (v:Ir.val): t :=
   mk ((regid, v)::c.(r)) c.(m) c.(s) c.(p) c.(cid_to_f) c.(cid_fresh).
+
+Definition update_m (c:t) (m:Ir.Memory.t): t :=
+  mk c.(r) m c.(s) c.(p) c.(cid_to_f) c.(cid_fresh).
 
 Definition get_funid (c:t) (cid:Ir.callid): option nat :=
   match (List.filter (fun x => Nat.eqb x.(fst) cid) c.(cid_to_f)) with
