Makefile
@@ -2,6 +2,8 @@ all:
 	coqc sflib.v
 	coqc Common.v
 	coqc Memory.v
+	coqc Value.v
 	coqc Lang.v
 	coqc State.v
 	coqc LoadStore.v WellTyped.v
+	coqc SmallStep.v
